fv/lean/Ragu/Circuits/Point/Double.lean
@@ -30,13 +30,13 @@ def main (input : Var Spec.Point (F p)) : Circuit (F p) (Var Spec.Point (F p)) :
 
   return ⟨x3, y3⟩
 
-def Assumptions (curveParams : Spec.CurveParams (F p)) (input : Spec.Point (F p)) :=
+def Assumptions (curveParams : Spec.CurveParams p) (input : Spec.Point (F p)) :=
   input.isOnCurve curveParams ∧
   -- for the circuit to be sound, there must not exist points of order 2 on the curve,
   -- therefore soundness is also conditioned on the following property:
   curveParams.noOrderTwoPoints
 
-def Spec (curveParams : Spec.CurveParams (F p)) (input : Spec.Point (F p)) (output : Spec.Point (F p)) :=
+def Spec (curveParams : Spec.CurveParams p) (input : Spec.Point (F p)) (output : Spec.Point (F p)) :=
   (match input.double with
   | none => False -- this case never happens
   | some double => output = double)
@@ -47,7 +47,7 @@ instance elaborated : ElaboratedCircuit (F p) Spec.Point Spec.Point where
   main
   localLength _ := 12
 
-theorem soundness (curveParams : Spec.CurveParams (F p)) : Soundness (F p) elaborated (Assumptions curveParams) (Spec curveParams) := by
+theorem soundness (curveParams : Spec.CurveParams p) : Soundness (F p) elaborated (Assumptions curveParams) (Spec curveParams) := by
   circuit_proof_start
   simp [circuit_norm,
     Element.Square.circuit, Element.Square.Assumptions, Element.Square.Spec,
@@ -81,10 +81,10 @@ theorem soundness (curveParams : Spec.CurveParams (F p)) : Soundness (F p) elabo
     exact h_d
 
 
-theorem completeness (curveParams : Spec.CurveParams (F p)) : Completeness (F p) elaborated (Assumptions curveParams) := by
+theorem completeness (curveParams : Spec.CurveParams p) : Completeness (F p) elaborated (Assumptions curveParams) := by
   sorry
 
-def circuit (curveParams : Spec.CurveParams (F p)) : FormalCircuit (F p) Spec.Point Spec.Point :=
+def circuit (curveParams : Spec.CurveParams p) : FormalCircuit (F p) Spec.Point Spec.Point :=
   {
     elaborated with
     Assumptions := Assumptions curveParams,
